soundness.v
@@ -7,6 +7,14 @@ Import ListNotations.
 
 (*Note: compile main.v before running this .v file *)
 
+(* the same ltac tactic to get the value from the option type in the DFA and the NFA built *)
+(* from a valid grammar.                                                                   *)
+
+Ltac grab_option x :=
+    match x with
+    | Some ?v => exact v
+    end.
+
 (* Lemmas about functions within the rhs module          *)
 Section rhs_lemmas.
 (*the following lemma states that isEmpty won't return a value different from false or true *)
@@ -25,6 +33,7 @@ Section rhs_lemmas.
   - intros. rewrite H. reflexivity.
   Qed.
 
+  (* Otherwise, it returns false iff the rule is not empty.                                   *)
   Lemma isEmpty_false : forall NT T, forall r:rhs.t T NT, rhs.isEmpty r = false <-> (r <> Empty).
   Proof.
   intros.
@@ -47,7 +56,13 @@ Section reg_grammar_lemmas.
   Proof.
   intros. unfold reg_grammar.build_grammar. reflexivity. Qed.
 
-  (*the following lemma states that the function step_rhs is sound                         *)
+  (* The following lemma states that the function step_rhs is sound. The step_rhs function checks if given *)
+  (* the RHS of a derivation rule and a terminal symbol, the rule can be used to derive this symbol.       *)
+  (* According to its definition, the resulting list is empty if the RHS is empty or the terminal symbol   *)
+  (* differs from the one that the RHS has.                                                                *)
+  (* This lemma states that for all executions of this function, it will return either an empty list,      *)
+  (* [None], which means a Rule "Single t" could be used or [Some nt], which means that a rule             *)
+  (* "Continue t nt" was used to derive the given "t"                                                      *)
   Lemma step_rhs_sound : forall t:T, forall rhs: rhs.t T NT, reg_grammar.step_rhs t rhs = [] \/
   reg_grammar.step_rhs t rhs = [None] \/ (exists nt, reg_grammar.step_rhs t rhs = [Some nt]).
   Proof.
@@ -84,7 +99,14 @@ Section reg_grammar_lemmas.
     rewrite e.  
   Admitted.*)
 
-  (*The following lemma states the soundness of the step_nt function. *)
+  (* The following lemma states the soundness of the step_nt function. This function tries to apply all    *)
+  (* the possible derivation rules for a given nonterminal symbol and a terminal symbol. It returns either *)
+  (* a empty list (if the terminal symbol being analyzed cannot be derived by the nonterminal symbol,      *)
+  (* a list that contains [None], which mean "there is a possible derivation from this nonterminal symbol" *)
+  (* "that uses the rule Single t, meaning this terminal symbol can be derived and the derivation can end" *)
+  (* or exists a nonterminal symbol that will be in the resulting list, meaning that a rule of the type    *)
+  (* "Continue t nt" could be used to derive the terminal symbol, being able to continue the derivation    *)
+  (* from "nt", which is another nonterminal symbol.                                                       *)
   Lemma step_nt_sound : forall rules,forall t, forall nt, reg_grammar.step_nt rules t nt =  [] \/
   In None (reg_grammar.step_nt rules t nt)  \/ (exists n:NT, In (Some n) (reg_grammar.step_nt rules t nt)).
   Proof.
@@ -94,7 +116,12 @@ Section reg_grammar_lemmas.
   - destruct o. right. right. simpl. exists n. left. reflexivity.
     right. left. simpl. left. reflexivity. Qed.
 
-  (*The following lemma states the soundness of the step function *)
+  (* The following lemma states the soundness of the step function. In other words, this function applies *)
+  (* "step_nt" to a list of possible nonterminal symbols, in which the derivation could be done. it works *)
+  (* just like the above function: an empty list is returned if in the list of nonterminal symbols, none  *)
+  (* of them can derive the given terminal symbol, a list containing at least None, which means there was *)
+  (* at least a RHS "Single t'" that could derive the t, or a list containing at least Some nt, where a   *)
+  (* rule of the kind "Continue t' nt" could be used to derive the terminal symbol t                      *)
   Definition step_sound: forall rules, forall t, forall acc, reg_grammar.step rules t acc = [] \/
   In (None) (reg_grammar.step rules t acc) \/ (exists nt:NT, In (Some nt)(reg_grammar.step rules t acc)).
   Proof.
@@ -105,9 +132,11 @@ Section reg_grammar_lemmas.
     right. left. simpl. left. reflexivity.
   Qed.
 
-  (*The following lemmas states the soundness of the parse' function, the main parser loop.*)
-  (*By the definition of parse', it should return or a empty list, or a list that has None *)
-  (*or a list that contains Some nt in it, some NT being a nonterminal symbol              *)
+  (* The following lemmas states the soundness of the parse' function, the main parser loop. By the      *)
+  (* definitionof parse', it should return or a empty list, or a list that has None or a list that       *)
+  (* or a list that contains Some nt in it, some NT being a nonterminal symbol. Recall that this function*)
+  (* will return a list of possible terminal symbols. works like the above function, but now for all the *)
+  (* terminal symbols given as input, it will try to apply valid rules on this list.                     *)
   Definition parse'_sound: forall rules, forall lt, forall lnt, reg_grammar.parse' rules lt lnt = [] 
   \/ In (None) (reg_grammar.parse' rules lt lnt) \/ (exists nt:NT, In (Some nt) (reg_grammar.parse' rules lt lnt)).
   Proof.
@@ -225,8 +254,10 @@ Section reg_grammar_lemmas.
   - intros. symmetry. rewrite <- H1. reflexivity.
   Qed. *)
 
-  (*this inductive proposition states when the parser for a given grammar in a list of *)
-  (*terminal symbols should return true. This comes straight from parse's definition. *)
+  (* This inductive proposition states when the parser for a given grammar in a list of terminal     *)
+  (* symbols should return true. This comes straight from parse's definition, where it should return *)
+  (* true if for all list of terminal symbols, from the starting symbol of the grammar, the parse'   *)
+  (* returns a accepting state (which means it was possible to derive this list.                     *)
   Inductive parse_true (g: reg_grammar.g T NT) : list T -> Prop :=
   | parse_t : forall l: list T,
                  ([Some (reg_grammar.start_symbol g)] |> reg_grammar.parse' (reg_grammar.rules g) l |> 
@@ -260,6 +291,22 @@ Section reg_grammar_lemmas.
   - intros. destruct H1. rewrite <- H1. reflexivity.
   Qed.
 
+  (* The following lemma states the soundness of the "get_nondetermism" function, which  *)
+  (* means: returns true iff there is at least a rule in the list of rules that goes to  *)
+  (* at least 2 different states in a given nonterminal symbol and with the same         *)
+  (* terminal symbol.                                                                    *)
+
+  (*
+  Lemma get_nondeterminism_true : forall rules, reg_grammar.get_nondeterminism rules rules
+  = true <-> (exists r:(NT * rhs.t T NT),
+  (reg_grammar.get_all_t rules (fst r) |> reg_grammar.count (reg_grammar.get_t_from_rhs(snd r))) >= 2).
+  Proof.
+  intros.
+  split.
+  - intros. destruct rules. inversion H1. exists p. inversion H1.
+  (* maybe it will be needed a indutcive proposition *)
+  *)
+
 
 End reg_grammar_lemmas.
 
@@ -292,49 +339,120 @@ Section dfa_lemmas.
   - intros. rewrite <- H1. reflexivity.
   Qed. *)
 
-  (* the following inductive proposition states that, after running a word in a automata built from a grammar, *)
-  (* if it reaches a final state, then we have the run of a given list of terminals on the automata is valid   *)
-  (* returns true                                                                                              *)
-  Inductive run_true (g: reg_grammar.g T NT) : list T -> Prop := 
-  |run_t : forall l:list T, 
-    (dfa.is_final (powerset_construction.dfa g)
-    (dfa.run' (dfa.next (powerset_construction.dfa g)) l
-     (dfa.initial_state (powerset_construction.dfa g))) = true)-> run_true g l.
+  (* The variable "x" below stands for a valid DFA:                                                 *)
+  Variable x : (dfa.t (powerset_construction.state NT) T).
+
+  (* The proposition "run_true" states that, given a valid DFA that can be built from a grammar,the       *)
+  (* powerset_construction.build_dfa returns a valid value (i.e, "Some a", where "a" has the same type as *)
+  (* the "x" presented above. Then, this given a returning true means that it reached a final state from a*)
+  (* given derivation that starts from the dfa's starting state.                                          *)
+  Inductive run_true_dfa (g: reg_grammar.g T NT) : list T -> Prop := 
+  |run_t : forall l:list T,
+   powerset_construction.build_dfa g = Some x /\
+  (dfa.is_final (x)
+    (dfa.run' (dfa.next (x)) l
+     (dfa.initial_state (x))) = true) -> run_true_dfa g l.
 
   (* The following lemma states that, for all runs on list of terminals for all automata built from a given grammar*)
   (* it retuns true iff it reaches a final state after running the word on the automata, starting in the initial   *)
   (*state of the automata, as stated in "run_true".                                                                 *)
-  Lemma run_soundness_true_forall: forall grammar:reg_grammar.g T NT, forall l:list T,
-  dfa.run (powerset_construction.dfa g) l = true  <-> run_true g l.
+  Lemma run_soundness_true_forall: forall g :reg_grammar.g T NT, forall l:list T,
+  powerset_construction.build_dfa g = Some x /\ dfa.run (x) l = true  <-> run_true_dfa g l.
   Proof.
   intros.
   split.
-  - intros. apply run_t. rewrite <- H1. reflexivity.
-  - intros. destruct H1. rewrite <- H1. reflexivity.
-  Qed.
+  - intros. apply run_t. destruct H1. split.
+    + rewrite <- H1. reflexivity.
+    + rewrite <- H2. reflexivity. 
+  - intros. destruct H1. destruct H1. split.
+    + assumption.
+    + rewrite <- H2. reflexivity. 
+  Qed. 
 
   (*Following the idea presented above, we can define the soundness in the case the automata *)
   (*should return false after a run in a given list of terminal symbols:                     *)
-  Inductive run_false (g: reg_grammar.g T NT) : list T -> Prop := 
-  |run_f : forall l:list T, 
-    (dfa.is_final (powerset_construction.dfa g)
-    (dfa.run' (dfa.next (powerset_construction.dfa g)) l
-     (dfa.initial_state (powerset_construction.dfa g))) = false)-> run_false g l.
+ Inductive run_false_dfa (g: reg_grammar.g T NT) : list T -> Prop := 
+  |run_f : forall l:list T,
+   powerset_construction.build_dfa g = Some x /\
+  (dfa.is_final (x)
+    (dfa.run' (dfa.next (x)) l
+     (dfa.initial_state (x))) = false) -> run_false_dfa g l.
 
-  Lemma run_soundness_false_forall: forall grammar:reg_grammar.g T NT, forall l:list T,
-  dfa.run (powerset_construction.dfa g) l = false  <-> run_false g l.
+  Lemma run_soundness_false_forall: forall g :reg_grammar.g T NT, forall l:list T,
+  powerset_construction.build_dfa g = Some x /\ dfa.run (x) l = false <-> run_false_dfa g l.
   Proof.
   intros.
   split.
-  - intros. apply run_f. rewrite <- H1. reflexivity.
-  - intros. destruct H1. rewrite <- H1. reflexivity.
-  Qed.
+  - intros.  destruct H1. apply run_f. split.
+    + rewrite <- H1. reflexivity.
+    + rewrite <- H2. reflexivity. 
+  - intros. destruct H1. destruct H1. split.
+    + assumption.
+    + rewrite <- H2. reflexivity. 
+  Qed. 
+
   (* Then, we can conclude that both the parser for a given grammar and the automata built from *)
   (* the same grammar does the same work. This is possible thanks to the way the automata's     *)
   (* behaviour is defined from a grammar.                                                       *)
-  Lemma dfa_and_parser : forall l, reg_grammar.parse g l = dfa.run (powerset_construction.dfa g) l.
+
+  (* ops
+  Lemma dfa_and_parser : forall l, 
+  ((powerset_construction.build_dfa g = Some x) /\ dfa.run (x) l)
+   = reg_grammar.parse g l.
     Proof.
+      intros.
+      unfold reg_grammar.parse.
       reflexivity.
-    Qed.
+    Qed. *)
 
 End dfa_lemmas.
+
+Section nfa_lemmas.
+  Variables (S A T NT : Type).
+  Variable g: reg_grammar.g T NT.
+  Context `{EqDec T eq} `{EqDec NT eq}.
+
+  (* Now it is presented the same idea, but for NFAs:                                           *)
+  Variable y: (nfa.t (powerset_construction_nfa.state NT) T).
+
+  Inductive run_true_nfa (g: reg_grammar.g T NT) : list T -> Prop := 
+  |run_t_nfa : forall l:list T,
+   powerset_construction_nfa.build_nfa g = Some y /\
+  (nfa.is_final (y)
+    (nfa.run' (nfa.next (y)) l
+     (nfa.initial_state (y))) = true) -> run_true_nfa g l.
+
+  Lemma run_soundness_true_forall_nfa: forall g :reg_grammar.g T NT, forall l:list T,
+  powerset_construction_nfa.build_nfa g = Some y /\ nfa.run (y) l = true  <-> run_true_nfa g l.
+  Proof.
+  intros.
+  split.
+  - intros. apply run_t_nfa. destruct H1. split.
+    + rewrite <- H1. reflexivity.
+    + rewrite <- H2. reflexivity. 
+  - intros. destruct H1. destruct H1. split.
+    + assumption.
+    + rewrite <- H2. reflexivity. 
+  Qed.
+
+  Inductive run_false_nfa (g: reg_grammar.g T NT) : list T -> Prop := 
+  |run_f_nfa : forall l:list T,
+   powerset_construction_nfa.build_nfa g = Some y /\
+  (nfa.is_final (y)
+    (nfa.run' (nfa.next (y)) l
+     (nfa.initial_state (y))) = false) -> run_false_nfa g l.
+
+  Lemma run_soundness_false_forall_nfa: forall g :reg_grammar.g T NT, forall l:list T,
+  powerset_construction_nfa.build_nfa g = Some y /\ nfa.run (y) l = false <-> run_false_nfa g l.
+  Proof.
+  intros.
+  split.
+  - intros. apply run_f_nfa. destruct H1. split.
+    + rewrite <- H1. reflexivity.
+    + rewrite <- H2. reflexivity. 
+  - intros. destruct H1. destruct H1. split.
+    + assumption.
+    + rewrite <- H2. reflexivity. 
+  Qed.
+
+End nfa_lemmas.
